type_system/type_lemmas.v
@@ -84,16 +84,20 @@ all: try unfold c_subs2_out.
 + destruct C as (A, Σ, E) eqn:e. apply shape_do in orig.
   destruct orig as [A' [c1ty]]. eapply c_subs_out_typesafe. eauto.
   apply shape_ret in c1ty. auto.
-+ destruct C as (A, Σ, E) eqn:e. apply shape_do in orig.
-  destruct orig as [A' [c1ty]]. eapply shape_op in c1ty.
-  destruct c1ty as [Aop [Bop [gets [vty]]]]. apply TypeC.
-  - inv H. inv H1. auto.
++ destruct C as (Ac, Σ, E) eqn:e. apply shape_do in orig.
+  destruct orig as [A' [c1ty]]. eapply shape_op_full in c1ty; eauto.
+  destruct c1ty as [vty[cty[Aop[Bop[gets[stya styb]]]]]]. apply TypeC.
+  - inv vty. auto.
   - inv H. auto.
-  - eapply TypeOp; eauto. eapply TypeC. inv H0. auto. inv H. auto.
-    eapply TypeDo. exact H0.
-    assert (CtxU (CtxU Γ Bop) A' = ctx_insert (CtxU Γ A') 1 Bop).
-    { simpl. destruct Γ; auto. }
-    rewrite H1. apply c_insert_typesafe. auto. inv H0. inv H2. auto.
+  - eapply TypeOp; eauto. 
+    * inv vty. auto.
+    * inv cty. inv H0. auto.
+    * eapply TypeC. inv cty. auto. inv H. auto.
+      eapply TypeDo; eauto.
+      assert (CtxU (CtxU Γ B) A' = ctx_insert (CtxU Γ A') 1 B) as same.
+      { simpl. destruct Γ; auto. }
+      rewrite same. apply c_insert_typesafe. auto.
+      inv cty. inv H0. auto.
 + eapply shape_handle in orig. destruct orig as [C' [hty]]. 
   apply TypeC. inv hty. auto. inv hty. inv H1. auto.
   eapply TypeHandle; eauto.
@@ -105,42 +109,46 @@ all: try unfold c_subs2_out.
   - inv hty. inv H2. auto.
   - eapply TypeCSubsume; eauto.
 + eapply shape_handle in orig. rename C into D. 
-  destruct orig as [C[hty]]. destruct C as (A, Σ, E).
+  destruct orig as [C[hty]]. destruct C as (Ac, Σ, E).
   eapply shape_handler in hty as hty'.
   destruct hty' as [Σ'[D'[retty[hcty[r[st]]]]]].
-  eapply shape_op in H0 as opt. destruct opt as [Aop[Bop[gets]]].
+  eapply shape_op_full in H0 as opt; eauto.
+  destruct opt as [vty[cty[Aop[Bop[gets[stya styb]]]]]].
   assert (wf_ctx Γ) by (inv hty; auto). 
-  apply TypeC; auto. inv hty. inv H5. auto.
-  eapply TypeCSubsume; eauto. inv H2.
-  assert (wf_vtype Aop) by (inv H4; auto).
-  assert (wf_vtype Bop) by (inv H5; inv H6; auto).
-  assert (wf_ctype D') by (inv hcty; auto).
+  apply TypeC; auto. inv hty. inv H4. auto.
+  eapply TypeCSubsume; eauto.
+  assert (wf_vtype A) as wfa by (inv vty; auto).
+  assert (wf_vtype B) as wfb by (inv cty; inv H3; auto).
+  assert (wf_ctype D') as wfd by (inv hcty; auto).
   eapply c_subs_out_typesafe.
-  instantiate (1:= Aop).
+  instantiate (1:= A).
   eapply c_subs_out_typesafe.
-  instantiate (1:= TyFun Bop D').
+  instantiate (1:= TyFun B D').
   - eapply sig_subtype_get_Some in gets; eauto.
-    destruct gets as [A'[B'[gets']]]. inv H8.
+    destruct gets as [A'[B'[gets']]]. inv H3.
     eapply ctx_subtype_ctype. eapply case_has_type; eauto.
     * apply WfCtxU. apply WfCtxU. 3: apply WfTyFun. all: auto.
     * apply STyCtxU. apply STyCtxU.
       apply ctx_subtype_refl; auto. auto.
-      apply STyFun; auto. apply csubtype_refl. all: auto.
-  - apply v_shift_typesafe. 2: (inv H4; auto).
+      eapply vsubtype_trans; eauto.
+      apply STyFun; auto. eapply vsubtype_trans; eauto. 
+      apply csubtype_refl. all: auto.
+  - apply v_shift_typesafe; auto.
     apply TypeV. auto. apply WfTyFun; auto.
     eapply TypeFun. apply TypeC. apply WfCtxU. all: auto.
-    eapply TypeHandle. 2: exact H5.
-    assert (CtxU Γ Bop = ctx_insert Γ 0 Bop) by (destruct Γ; simpl; auto).
-    rewrite H8. eapply v_insert_typesafe. 2: auto.
+    eapply TypeHandle. 2: eauto.
+    assert (CtxU Γ B = ctx_insert Γ 0 B) as same by (destruct Γ; simpl; auto).
+    rewrite same. eapply v_insert_typesafe. 2: auto.
     apply TypeV. auto. apply WfTyHandler. inv H0. auto. auto.
-    eapply TypeVSubsume. instantiate (1:=(TyHandler (CTy A Σ' E) D'));
-    inv H5; inv H10; inv H0.
-    * apply TypeV. auto. apply WfTyHandler. apply WfCTy; auto.
-      all: try (inv hcty; assumption). eapply wf_eqs_sig_subtype; eauto.
-      inv hcty. auto. apply TypeHandler; auto.
-    * apply STyHandler. apply STyCTy. 2: auto.
-      apply vsubtype_refl. inv H5. inv H10. auto.
-      eapply eqs_subtype_refl. inv H5. inv H10. eauto.
+    assert (wf_sig Σ') as wfsig by (inv hcty; auto).
+    eapply TypeVSubsume. instantiate (1:=(TyHandler (CTy Ac Σ' E) D')).
+    * inv H0. inv H4.
+      apply TypeV. auto. apply WfTyHandler; auto. apply WfCTy; auto.
+      eapply wf_eqs_sig_subtype; eauto. apply TypeHandler; auto.
+    * inv H0. inv H4.
+      apply STyHandler. apply STyCTy. 2: auto.
+      apply vsubtype_refl. inv cty. inv H4. auto.
+      eapply eqs_subtype_refl; eauto.
       apply csubtype_refl. auto.
   - auto.
 Qed.
@@ -150,7 +158,7 @@ Qed.
 Theorem progress c C:
   has_ctype CtxØ c C ->
   (exists v, c = Ret v) \/
-  (exists o v c', c = Op o v c') \/
+  (exists o A B v c', c = Op o A B v c') \/
   (exists c', step c c'). 
 Proof.
 revert C. induction c; intros C orig.
@@ -189,14 +197,14 @@ revert C. induction c; intros C orig.
   - destruct H0 as [n same]. rewrite same in *.
     apply shape_var_ctx_empty in fty. destruct fty.
   - destruct H0 as [x [c [same]]]. subst. eexists. apply Step_AppFun.
-+ right. left. eauto.
++ right. left. exists o, v, v0, v1, c. auto.
 + right. right. clear IHc1 IHc2.
   eexists. apply Step_LetRecStep.
 + right. right. clear IHc2. destruct C as (A, Σ, E). 
   eapply shape_do in orig. destruct orig as [A' [c1ty]].
   apply IHc1 in c1ty as IH. clear IHc1. destruct IH as [h1 | [h2 | h3]].
   - destruct h1. rewrite H0 in *. eexists. apply Step_DoRet.
-  - destruct h2. destruct H0. destruct H0 as [c' same]. rewrite same in *.
+  - destruct h2. destruct H0 as [Aop[Bop[v[c same]]]]. rewrite same in *.
     eexists. apply Step_DoOp.
   - destruct h3. eexists. apply Step_DoStep. exact H0.
 + right. right. eapply shape_handle in orig. rename C into D.
@@ -208,8 +216,10 @@ revert C. induction c; intros C orig.
   destruct H0 as [c_r[h[Σ'[D'[same[crty]]]]]]. subst.
   destruct H'. 2: destruct H1.
   - destruct H1 as [v]. subst. eexists. apply Step_HandleRet.   
-  - destruct H1 as [op[v[c']]]. subst. destruct H0 as [hcsty[r[sigsty]]].
-    apply shape_op in H. destruct H as [A_op[B_op[gets]]].
+  - destruct H1 as [op[Aop[Bop[v[c']]]]]. subst.
+    destruct H0 as [hcsty[r[sigsty]]].
+    eapply shape_op_full in H; eauto.
+    destruct H as [vty[cty[A_op[B_op[gets _]]]]].
     eapply sig_subtype_get_Some in gets. 2: exact sigsty.
     destruct gets as [A'[B'[gets']]].
     eapply h_has_case in hcsty. 2: exact gets'.
